\documentclass{article}
\usepackage{graphicx} % Required for inserting images
\usepackage[top=0.9in, bottom=1in, left=1.5in, right=1.5in]{geometry}
\usepackage[utf8]{inputenc}
\usepackage[icelandic]{babel}
\usepackage[T1]{fontenc}
\usepackage[sc]{mathpazo}
\usepackage[parfill]{parskip}
\renewcommand{\baselinestretch}{1.2}
% Tables and lists
\usepackage{booktabs,tabularx}
\usepackage{multirow}
\usepackage{enumerate}
\usepackage{adjustbox}
\usepackage{multicol}
\usepackage{xcolor}
\usepackage{algpseudocode}
\usepackage{tikz}
\usepackage{nicefrac}
\usepackage{changepage}
\usetikzlibrary{arrows, positioning, calc, graphs}

% Math
\usepackage{amsmath, amsfonts, amssymb, amsthm}
% Graphics

\usepackage{graphicx}
\usepackage{tikz}
% Code environment
\usepackage{minted}
%\usepackage{bm}
%\usepackage{siunitx}
%\usepackage{animate}
%\usepackage{hyperref}
%\usepackage{movie15}
%\usepackage{multicol}
%\usepackage{changepage}
\title{Formal Languages and Computability 5}
\author{Ragnar BjÃ¶rn Ingvarsson, rbi3}
\tikzset{->, >=stealth', shorten >=1pt, node distance=2cm,thick, main node/.style={circle,draw,minimum size=3em}}


\begin{document}
\renewcommand\thepage{}
	
	\maketitle

	\newpage
	\setcounter{page}{1}
	\renewcommand\thepage{\arabic{page}}

	\section{The DFA depicted below determines whether the remainder after 
		dividing a \textit{binary number} by three is one. Convert it to 
		a corresponding context-free grammar.}

		We will use the algorithm described in lecure 5.

		There are three states so we will get variables $R_0$, $R_1$ and 
		$R_2$. Then we get the rules

		$R_0 \rightarrow 0R_0 \hspace{.5em} | \hspace{.5em} 1R_1$ \\
		$R_1 \rightarrow 1R_0 \hspace{.5em} | \hspace{.5em} 0R_2 \hspace{.5em} | \hspace{.5em} \epsilon$ \\
		$R_2 \rightarrow 1R_2 \hspace{.5em} | \hspace{.5em} 0R_1$

		Where the start variable is $R_0$.

	\section{Convert the following CFG into an equivalent CFG in Chomsky 
		normal form, using the procedure given in Theorem 2.9}

		We start with

		\[A\rightarrow BAB\mid B\mid\epsilon\]
		\[B\rightarrow 00\mid\epsilon\]

		And then we first add a start state $S_0$ and rule $S_0\rightarrow 
		A$. Then we remove all $\epsilon$-rules by adding a case to all 
		rules which contain the nullable variable on the right hand side 
		where the nullable variable does not occur.

		We start with $B$ and get

		\[S_0\rightarrow A\]
		\[A\rightarrow BAB\mid BA\mid AB\mid B\mid \epsilon\]
		\[B\rightarrow 00\]

		And then do $A$ as well:

		\[S_0\rightarrow A\mid \epsilon\]
		\[A\rightarrow BAB\mid BA\mid AB\mid B\]
		\[B\rightarrow 00\]

		We then get rid of unit rules:

		\[S_0\rightarrow BAB\mid BA\mid AB\mid 00\mid \epsilon\]
		\[A\rightarrow BAB\mid BA\mid AB\mid 00\]
		\[B\rightarrow 00\]

		We then remove the long rules:

		\[S_0\rightarrow BA_1\mid BA\mid AB\mid 00\mid \epsilon\]
		\[A\rightarrow BA_1\mid BA\mid AB\mid 00\]
		\[B\rightarrow 00\]
		\[A_1\rightarrow AB\]

		And then at last we remove the excess terminal symbols with

		\[S_0\rightarrow BA_1\mid BA\mid AB\mid U_1U_1\mid \epsilon\]
		\[A\rightarrow BA_1\mid BA\mid AB\mid U_1U_1\]
		\[B\rightarrow U_1U_1\]
		\[A_1\rightarrow AB\]
		\[U_1\rightarrow 0\]

		And now we are done. As we can see, the CFG is in Chomsky normal 
		form as all rules are of the form $A\rightarrow BC$ or 
		$A\rightarrow a$ or $S\rightarrow\epsilon$.

		\section{}

		\begin{itemize}
			\item[a)] We can give the CFG with the start state $S$:

					\[S\rightarrow 0BA0\]
					\[A\rightarrow 0A0\mid \geq\]
					\[B\rightarrow 0B\mid \epsilon\]
			\item[b)] We define the start state to be $S$ again:

				\[S\rightarrow 0A0\]
				\[A\rightarrow B0C0\mid 0A0\]
				\[B\rightarrow 0B\mid B0\mid +\]
				\[C\rightarrow 0C0\mid \geq\]
			\item[c)] If $i_A = i_B$ and so forth, then $A\cup B$ is not 
				CF since then it would be impossible to ensure that in 
				both $A$ and $B$ there are the same amount of $0$'s in one 
				place and not in some other, but if $i_A$ is unrelated to 
				$i_B$ and so on, the language $C= A\cup B$ is indeed CF 
				since we can just add the start state $S_0$ and rule 
				$S_0 \rightarrow S_AS_B$ where $S_A$ is the start state for 
				$A$ and $S_B$ is the start state for $B$. 
		\end{itemize}

\end{document}
